LeanBoogie/ITree.lean
@@ -2,6 +2,6 @@ import LeanBoogie.ITree.ITree
 import LeanBoogie.ITree.Monad
 import LeanBoogie.ITree.Iter
 import LeanBoogie.ITree.RunFinite
-import LeanBoogie.ITree.Events
+import LeanBoogie.ITree.Effect
 import LeanBoogie.ITree.Eutt
 import LeanBoogie.ITree.Imp
