LeanBoogie/ITree/Effect.lean
@@ -1,0 +1,76 @@
+import LeanBoogie.ITree.ITree
+import LeanBoogie.ITree.Iter
+
+namespace ITree
+
+/-
+  # Effects
+-/
+
+-- /-- Just a tag. -/
+-- class IsEffect (E : Type -> Type)
+
+/-- No effects. This is essentially `Empty`. -/
+def None : Type -> Type := fun _ => PEmpty
+instance : Inhabited (Type -> Type) := ⟨None⟩
+instance : EmptyCollection (Type -> Type) := ⟨None⟩
+
+instance : OfNat (Type -> Type) 0 where ofNat := None
+
+/-- The union of two event types. -/
+inductive Effect.Prod (E₁ E₂ : Type -> Type) : Type -> Type
+| left  : E₁ Ans -> Prod E₁ E₂ Ans
+| right : E₂ Ans -> Prod E₁ E₂ Ans
+
+def Effect.NProd (Es : List (Type -> Type)) : (Type -> Type) :=
+  fun Ans => (i : Fin Es.length) -> Es[i] Ans
+
+-- Maybe `Union` would be better?
+-- instance : Add Effect := ⟨Effect.Prod⟩
+-- instance : Add (Type -> Type) := ⟨Effect.Prod⟩
+infix:30 " & " => Effect.Prod
+
+#check None & None
+
+/-- Asserts that the collection of events `Es` has event `E`.
+
+  Note: Usage of this typeclass in conjunction with `Effect.Prod` seems a little buggy, I haven't
+  gotten around to why it is wonky yet.
+-/
+class HasEff (E : semiOutParam (Type -> Type)) (Es : Type -> Type) where
+  inj : {Ans : Type} -> E Ans -> Es Ans
+  /-- The rest of the events in `Es`, without `E`. -/
+  Strip : Type -> Type
+  elim : {Ans : Type} -> {motive : Type} -> (E Ans -> motive) -> (Strip Ans -> motive) -> Es Ans -> motive
+
+instance instCoeEff {E Es : Type -> Type} [HasEff E Es] {Ans : Type} : Coe (E Ans) (Es Ans)
+  := ⟨HasEff.inj⟩
+attribute [coe] HasEff.inj
+
+instance (priority := low) instHasEff_id {E : Type -> Type} : HasEff E E where
+  inj := id
+  Strip := None
+  elim l _ := l
+
+instance instHasEff_left {E₁ E₂ : Type -> Type} : HasEff E₁ (E₁ & E₂) where
+  inj := .left
+  Strip := E₂
+  elim l r := fun | .left e1 => l e1 | .right e2 => r e2
+
+instance instHasEff_right {E₁ E₂ : Type -> Type} : HasEff E₂ (E₁ & E₂) where
+  inj := .right
+  Strip := E₁
+  elim l r := fun | .left e1 => r e1 | .right e2 => l e2
+
+/-
+  # Interp, Handlers
+
+  The ITree paper just defines one `interp` using `iter`, for which you can then obtain concrete
+  interpretations by giving it a `handler`.
+  I wasn't able to figure out how `iter` is supposed to be used here. The code in the ITree repo
+  is slightly different from the code in the paper.
+-/
+
+-- def interp  [Monad M] (handler : {A : Type} -> E A -> M A)
+--   : ITree E A -> M A
+--   := fun t => iter (fun t => sorry)
