LeanBoogie/Iter.lean
@@ -1,9 +1,12 @@
 import LeanBoogie.Notation
 
+namespace LeanBoogie
+
 /-- The monad `M` is equipped with `iter`. -/
 class Iter (M : Type u -> Type v) [Monad M] where
   iter : {A B : Type u} -> (A -> M (A ⊕ B)) -> A -> M B
-open Iter
+
+export Iter (iter)
 
 -- class LawfulIter (M : Type -> Type) {equiv : {A : Type} -> M A -> M A -> Prop} [Monad M] [Iter M] : Prop where
 --   iter_fp : equiv (iter f a) (iter f a)
