LeanBoogie/MRec.lean
@@ -1,0 +1,53 @@
+import LeanBoogie.ITree
+import LeanBoogie.State
+import Mathlib.Data.Real.Basic
+
+namespace LeanBoogie
+open ITree (Effect HasEff)
+
+
+/-
+  # MRec
+  Self-recursion and mutual recursion.
+
+  See section 3.3 of the [ITree paper](https://dl.acm.org/doi/pdf/10.1145/3371119).
+-/
+
+-- Approach 1:
+-- inductive MRec (P : Con) : Type -> Type
+-- | call : Var P (A ~> B) -> A -> MRec P B
+-- def call [HasEff (MRec P) Es] (p : Var P (.map A B)) (a : A) : ITree Es B :=
+--   .vis (MRec.call p a) .ret
+-- def rec
+--   (procs : Var P (X ~> Y) -> X -> ITree (Mem Γ + MRec P) Y)
+--   (main : ITree (Mem Γ + MRec P) A)
+--   : ITree (Mem Γ) A
+--   := sorry -- ...iter...
+-- structure Proc where
+--   A : Type
+--   B : Type
+
+inductive MRec {Proc : Type} (pTys : Proc -> Type × Type) : Type -> Type
+| call : (p : Proc) -> (pTys p).1 -> MRec pTys (pTys p).2
+
+def call {Proc} (P : Proc -> Type × Type) [HasEff (MRec P) E] (p : Proc) (a : (P p).1) : ITree E (P p).2 :=
+  .vis (MRec.call p a) .ret
+
+/-- This `mrec` is very different from the ITree paper. -/
+def mrec {E : Type -> Type} {Proc} (P)
+  (p : Proc)
+  (procs : (p : Proc) -> (P p).1 -> ITree (E + MRec P) (P p).2)
+  : (P p).1 -> ITree E (P p).2
+  := ITree.iter (fun ab => sorry) -- probably a bad idea actually, go with the ITree paper approach instead?
+
+-- Example:
+inductive Procs | f | g
+def P : Procs -> Type × Type | _ => ⟨Int, Int⟩
+
+def mutualBlock : Int -> ITree E Int := mrec P Procs.f fun
+| Procs.f, (x : Int) => do -- def of `f`
+  let n : Int <- call P .g (x * 3) -- `g(x * 3)`
+  return n
+| Procs.g, (x : Int) => do -- def of `g`
+  let n : Int <- call P .f (x / 2) -- `f(x / 2)`
+  return - n
