LeanBoogie/State.lean
@@ -1,0 +1,161 @@
+import LeanBoogie.Mem
+import LeanBoogie.Iter
+
+namespace LeanBoogie
+
+/-
+  The file `Mem.lean` only defines the `Mem` effect, but lacks any interpretation.
+  We give one interpretation here.
+
+  You can imagine giving a completely different model for memory events in a world without
+  strong consistency guarantees. I have no idea how that would look like, but it would
+  be very interesting to try.
+-/
+
+/-
+  # The state monad
+-/
+
+/-- E.g. `ConA [.int, .bv 32] ≣ Unit × Int × BitVec 32`. -/
+abbrev ConA : Con -> Type
+| [] => Unit
+| x :: xs => TyA x × ConA xs
+
+instance : CoeSort Con Type := ⟨ConA⟩
+
+set_option linter.unusedVariables false in
+/-- Read a variable's value from the state. -/
+def ConA.get : {Γ : Con} -> Γ -> Var Γ A -> A
+| _ :: _, (x, _), .vz   => x
+| _ :: _, (_, γ), .vs v => γ.get v
+
+set_option linter.unusedVariables false in
+/-- Set a variable's value, returning an updated state.
+  Example: `γ.set v 123 : Γ`.  -/
+def ConA.set : {Γ : Con} -> Γ -> Var Γ A -> A -> Γ
+| _ :: _, (_, γ), .vz  , a' => (a', γ)
+| _ :: _, (a, γ), .vs v, a' => (a, γ.set v a')
+
+def State.read [Monad M] (v : Var Γ A) : StateT Γ M A := fun γ => return (γ.get v, γ)
+def State.write [Monad M] (v : Var Γ A) (val : A) : StateT Γ M PUnit := fun γ => return (.unit, γ.set v val)
+
+-- def State.iter [Monad M] [Iter M] {Γ A : Type} (f : A -> Γ -> M ((A ⊕ B) × Γ)) (a₀ : A) : Γ -> M (B × Γ) :=
+def State.iter [Monad M] [Iter M] /- {Γ : Con} -/ (f : A -> StateT Γ M (A ⊕ B)) (a₀ : A) : StateT Γ M B :=
+  fun γ => Iter.iter (fun (⟨a, γ⟩ : A × Γ) => do
+    let ⟨ab, γ'⟩ <- f a γ
+    match ab with
+    | .inl (a : A) => return .inl ⟨a, γ'⟩ -- continue
+    | .inr (b : B) => return .inr ⟨b, γ'⟩ -- done
+  ) (a₀, γ)
+
+instance [Monad M] [Iter M] : Iter (StateT Γ M) := ⟨State.iter⟩
+
+/-
+  ## Equational reasoning for our state monad
+
+  The above `interp_*` lemmas show that `interp` is a monad morphism.
+  We should also show properties about the interpreted state, which we can not show on the `Mem` events.
+  For example, last write wins, etc.
+-/
+
+/- ### Normal form of `ConA`
+  Given a starting `γ : ConA Γ` and `γ' = γ.update |>.update .. |>.update ... |> ...`,
+  we can normalize these into essentially `γ' = { #0 := ...γ..., #1 := ...γ..., #2 := ...γ..., ...}`.
+
+  - We should eventually have a tactic which performs this normalization in a performant way.
+  - We should eventually have a delaborator which can render states `γ : ConA Γ` in a more
+    human-readable way.
+-/
+
+@[simp] theorem ConA.update_lww {Γ : Con} {v : Var Γ A} {γ : Γ} : (γ.set v a').set v a'' = γ.set v a'' := sorry
+@[simp] theorem ConA.update_get {Γ : Con} {v : Var Γ A} {γ : Γ} : (γ.set v a').get v = a' := by
+  induction Γ with
+  | nil => cases v
+  | cons B Γ ih =>
+    cases v with
+    | vz => rfl
+    | vs v => simp only [get, ih]
+-- more theorems
+
+
+
+
+
+
+
+
+/-
+  # Interpreting
+-/
+
+def interp (tm : ITree (Mem Γ) A) : StateT Γ (ITree ∅) A := fun s₀ =>
+  ITree.corec (fun ⟨tm, s⟩ =>
+    match tm.dest with
+    | .ret (.up a) => .ret (.up (a, s))
+    | .tau t => .tau (t, s)
+    | .vis ⟨Ans, .up ((e : Mem Γ Ans)), (k : ULift Ans -> ITree (Mem Γ) A)⟩ =>
+      match e with
+      | .rd v => .tau ⟨k (.up (s.get v)), s⟩
+      | .wr v val => .tau ⟨k (.up ()), s.set v val⟩
+  ) (tm, s₀)
+
+def interp' {E : Type -> Type} (tm : ITree (E & Mem Γ) A) : StateT Γ (ITree E) A := fun s₀ =>
+  ITree.corec (fun ⟨tm, s⟩ =>
+    match tm.dest with
+    | .ret (.up a) => .ret (.up (a, s))
+    | .tau t => .tau (t, s)
+    | .vis ⟨Ans, .up (.left  (e : E Ans    )), k⟩ => .vis ⟨Ans, .up e, fun ans => ⟨k ans, s⟩⟩ -- don't interpret the rest of the effects.
+    | .vis ⟨Ans, .up (.right (e : Mem Γ Ans)), (k : ULift Ans -> ITree (E & Mem Γ) A)⟩ =>
+      match e with
+      | .rd v => .tau ⟨k (.up (s.get v)), s⟩
+      | .wr v val => .tau ⟨k (.up ()), s.set v val⟩
+  ) (tm, s₀)
+
+-- Ideally we want something as general as this:
+-- def interp'' {E : Type -> Type} [inst : HasEff (Mem Γ) E] (tm : ITree E A) : StateT Γ (ITree inst.Strip) A := fun s₀ =>
+--   ITree.corec (fun ⟨tm, s⟩ =>
+--     match tm.dest with
+--     | .ret (.up a) => .ret (.up (a, s))
+--     | .tau t => .tau (t, s)
+--     | .vis ⟨Ans, .up ((e : E Ans    )), k⟩ =>
+--       inst.elim (fun e =>
+--         match e with
+--         | .rd v => .tau ⟨k (.up (s.get v)), s⟩
+--         | .wr v val => .tau ⟨k (.up ()), s.set v val⟩
+--       ) (fun e => .vis e k) e
+--   ) (tm, s₀)
+
+theorem interp_pure : interp (pure a : ITree (Mem Γ) A) = pure a := sorry
+
+theorem interp_bind {ta : ITree (Mem Γ) A} {tb : A -> ITree (Mem Γ) B}
+  : interp (ta >>= tb) = (interp ta) >>= (fun a => interp (tb a))
+  := sorry
+
+-- /-- Convenience mix of `interp_bind` and `bind_state_pull`. -/
+theorem interp_bind_pull {ta : ITree (Mem Γ) A} {tb : A -> ITree (Mem Γ) B}
+  : interp (bind ta tb) s = bind (interp ta s) (fun x => interp (tb x.1) x.2)
+  := sorry
+
+theorem interp_iter {f : A -> ITree (Mem Γ) (A ⊕ B)} {a₀ : A}
+  : interp (iter f a₀) = iter (fun (a : A) => interp (f a)) a₀
+  := sorry
+
+theorem interp_read {v : Var Γ A} : interp (Mem.read v) = State.read v := sorry
+theorem interp_write {v : Var Γ A} : interp (Mem.write v val) = (State.write v val) := sorry
+theorem interp_ite [Decidable φ] : interp (if φ then t else e) = (if φ then interp t else interp e) := sorry
+
+
+
+-- ## Example:
+
+structure Global_ where
+  i : Int
+  n : BitVec 32
+
+def Global.Γ : Con := [.int, .bv 32]
+abbrev Global : Type := Global.Γ
+abbrev Global.i (γ : Global) : Int       := γ.get .vz
+abbrev Global.n (γ : Global) : BitVec 32 := γ.get (.vs .vz)
+
+#check Global_.i
+#check Global.i
